include/s2n-bignum.h
@@ -743,6 +743,11 @@ extern void curve25519_pxscalarmul_alt(uint64_t res[static 8],uint64_t scalar[st
 extern void curve25519_x25519(uint64_t res[static 4],uint64_t scalar[static 4],uint64_t point[static 4]);
 extern void curve25519_x25519_alt(uint64_t res[static 4],uint64_t scalar[static 4],uint64_t point[static 4]);
 
+// x25519 function for curve25519 on base element 9
+// Input scalar[4]; output res[4]
+extern void curve25519_x25519base(uint64_t res[static 4],uint64_t scalar[static 4]);
+extern void curve25519_x25519base_alt(uint64_t res[static 4],uint64_t scalar[static 4]);
+
 // Extended projective + precomputed mixed addition for edwards25519
 // Inputs p1[16], p2[12]; output p3[16]
 extern void edwards25519_pepadd(uint64_t p3[static 16],uint64_t p1[static 16],uint64_t p2[static 12]);
